src/high/recovery_weakestpre.v
@@ -1,10 +1,12 @@
 (* Implementation of the recovery weakest precondition for NvmLang. *)
 From Perennial.program_logic Require Import crash_weakestpre.
-From Perennial.program_logic Require recovery_weakestpre.
+From Perennial.program_logic Require Import recovery_weakestpre.
+From Perennial.program_logic Require Import recovery_adequacy.
 
 From self Require Import view.
 From self.base Require Import primitive_laws wpr_lifting.
-From self.high Require Import dprop weakestpre crash_weakestpre.
+From self.high Require Import dprop.
+From self.high Require Import weakestpre crash_weakestpre.
 
 Set Default Proof Using "Type".
 
@@ -12,14 +14,7 @@ Notation pbundleG := recovery_weakestpre.pbundleG.
 
 Notation perennialG := recovery_weakestpre.perennialG.
 
-(* A recovery WP is parameterized by three predicates: [Φ] is the postcondition
-   for normal non-crashing execution. [Φr] is the postcondition satisfied in
-   case of a crash. Finally, [Φinv] is a condition that holds at each restart
-   point. *)
-Check expr_wpc.
-
-(* This approach does not seem to work. *)
-(*
+(* This approach does not seem to work.
 Definition wpr `{hG : !nvmG Σ} `{hC : !crashG Σ} (s : stuckness) (k : nat) E
            (e : expr) (rec : expr) (Φ : val → dProp Σ) (Φinv : nvmG Σ → dProp Σ) (Φc : nvmG Σ -> val -> dPropO Σ) :=
   MonPred (λ V,
@@ -36,47 +31,75 @@ Definition wpr `{hG : !nvmG Σ} `{hC : !crashG Σ} (s : stuckness) (k : nat) E
         (λ _, True%I)
         (λ hG res,
           let '(ThreadVal v TV') := res in Φc (hG) v TV')
-  )%I.
-*)
+  )%I. *)
 
-Definition wpr_pre `{nvmG Σ} `{hC : !crashG Σ} (s : stuckness) (k : nat)
+Record nvm_high_names := {
+  name_abs_history : gname;
+  name_predicates : gname;
+}.
+
+Definition nvm_high_get_names Σ (hG : nvmHighG Σ) : nvm_high_names :=
+  {| name_abs_history := abs_history_name;
+     name_predicates := predicates_name |}.
+
+Canonical Structure nvm_high_namesO := leibnizO nvm_high_names.
+
+(** Given an [hG : nvmG Σ], update the fields per the information in the rest of
+the arguments. In particular, all the gnames in [names] replaces the
+corresponding gnames in [hG]. *)
+Definition nvm_high_update Σ (hG : nvmHighG Σ) (names : nvm_high_names) :=
+  {| abs_history_name := names.(name_abs_history);
+     predicates_name := names.(name_predicates);
+     ra_inG := hG.(@ra_inG _);
+     ra'_inG := hG.(@ra'_inG _); |}.
+
+Record nvm_names := {
+  name_base_names : nvm_base_names; (* Names used by the base logic. *)
+  name_high_names : nvm_high_names; (* Names used by the high-level logic. *)
+}.
+
+Definition nvm_get_names Σ (hG : nvmG Σ) : nvm_names :=
+  {| name_base_names := nvm_base_get_names _ nvmG_baseG;
+     name_high_names := nvm_high_get_names _ nvmG_highG |}.
+
+Canonical Structure nvm_namesO := leibnizO nvm_names.
+
+(** Given an [hG : nvmG Σ], update the fields per the information in the rest of
+the arguments. In particular, all the gnames in [names] replaces the
+corresponding gnames in [hG]. *)
+Definition nvm_update Σ (hG : nvmG Σ) (Hinv : invG Σ) (Hcrash : crashG Σ) (names : nvm_names) :=
+  {| nvmG_baseG := nvm_base_update _ hG.(@nvmG_baseG _) Hinv Hcrash names.(name_base_names);
+     nvmG_highG := nvm_high_update _ hG.(@nvmG_highG _) names.(name_high_names) |}.
+
+(* The recovery WP is parameterized by two predicates: [Φ] is the postcondition
+   for normal non-crashing execution and [Φr] is the postcondition satisfied in
+   case of a crash. *)
+Definition wpr_pre Σ (s : stuckness) (k : nat)
     (wpr : crashG Σ -d> nvmG Σ -d> coPset -d> expr -d> expr -d> (val -d> dPropO Σ) -d>
                      (nvmG Σ -d> val -d> dPropO Σ) -d> dPropO Σ) :
   crashG Σ -d> nvmG Σ -d> coPset -d> expr -d> expr -d> (val -d> dPropO Σ) -d>
-  (crashG Σ -d> nvmG Σ -d> val -d> dPropO Σ) -d> dPropO Σ :=
-  λ Hc0 t0 E e rec Φ Φr,
+  (nvmG Σ -d> val -d> dPropO Σ) -d> dPropO Σ :=
+  λ Hc hG E e rec Φ Φr,
   (WPC e @ s ; k; E
      {{ Φ }}
-     {{ ∀ σ σ' (HC: crash_prim_step _ σ σ') n,
-        ⎡ interp -∗ state_interp σ n ={E}=∗ ▷ ∀ Hc1 q, NC q ={E}=∗
-          ∃ names,
-            let hG := (nvm_update _ _ _ Hc1 (@recovery_weakestpre.pbundleT _ _ names)) in
-            state_interp σ 0 ∗
-            wpr Hc1 hG E rec rec (λ v, Φr hG v) Φinv Φr
-            NC q ⎤
+     {{ ∀ σ σ' (HC: crash_prim_step nvm_crash_lang σ σ') n,
+        ⎡ interp -∗ state_interp σ n ={E}=∗ ▷ ∀ (Hc1 : crashG Σ) q, NC q ={E}=∗
+          ∃ (names : nvm_names),
+            let hG := (nvm_update _ hG _ Hc names) in
+              state_interp σ 0 ∗
+              (monPred_at (wpr Hc1 hG E rec rec (λ v, Φr hG v) Φr) (∅, ∅, ∅)) ∗
+              NC q ⎤
           }})%I.
-        True
-     }})%I.
-        (* ⎡interp -∗ global_state_interp g ns κs ={E}=∗  ▷ ∀ Hc1 q, NC q ={E}=∗ ∃ t1 *)
-        (*     (Hsame_inv: @iris_invG _ _ (recovery_weakestpre.perennial_irisG Hc1 t1) = *)
-        (*                 @iris_invG _ _ (recovery_weakestpre.perennial_irisG Hc0 t0)), *)
-        (*   □ (∀ g ns κs, @global_state_interp _ _ (recovery_weakestpre.perennial_irisG Hc1 t1) g ns κs ∗-∗ *)
-        (*                 @global_state_interp _ _ (recovery_weakestpre.perennial_irisG Hc0 t0) g ns κs) ∗ *)
-        (*   state_interp σ' 0 ∗ *)
-        (*   global_state_interp g (S ns) κs ∗ *)
-        (*   (monPred_at (wpr Hc1 t1 E rec rec (λ v, Φr Hc1 t1 v) Φr) ⊥) ∗ NC q⎤}})%I. *)
 
-Local Instance wpr_pre_contractive `{!nvmG Σ} s k: Contractive (wpr_pre s k).
+Local Instance wpr_pre_contractive {Σ} s k: Contractive (wpr_pre Σ s k).
 Proof.
-  rewrite /wpr_pre=> n wp wp' Hwp H2crash t E1 e1 rec Φ Φinv Φc.
+  rewrite /wpr_pre. intros ??? Hwp ???????.
   apply wpc_ne; eauto;
   repeat (f_contractive || f_equiv). apply Hwp.
 Qed.
 
-Definition wpr_def `{!perennialG Λ CS T Σ} (s : stuckness) k :
-  crashG Σ → pbundleG T Σ → coPset → expr Λ → expr Λ → (val Λ → iProp Σ) →
-  (crashG Σ → pbundleG T Σ → iProp Σ) →
-  (crashG Σ → pbundleG T Σ → val Λ → iProp Σ) → iProp Σ := fixpoint (wpr_pre s k).
-Definition wpr_aux `{!perennialG Λ CS T Σ} : seal (@wpr_def Λ CS T Σ _). by eexists. Qed.
-Definition wpr `{!perennialG Λ CS T Σ} := wpr_aux.(unseal).
-Definition wpr_eq `{!perennialG Λ CS T Σ} : wpr = @wpr_def Λ CS T Σ _ := wpr_aux.(seal_eq).
+Definition wpr_def {Σ} (s : stuckness) k := fixpoint (wpr_pre Σ s k).
+
+Definition wpr_aux {Σ} : seal (@wpr_def Σ). by eexists. Qed.
+
+Definition wpr `{nvmG Σ} s k := wpr_aux.(unseal) s k _ _.
