src/high/crash_weakestpre.v
@@ -1,4 +1,6 @@
+From iris.proofmode Require Import base tactics classes.
 From Perennial.program_logic Require crash_weakestpre.
+
 From self.high Require Export dprop.
 From self.base Require Import primitive_laws.
 From self.high Require Import weakestpre.
@@ -8,7 +10,7 @@ Section wpc.
 
   Program Definition wpc_def s k E e (Φ : val → dProp Σ) (Φc : dProp Σ) : dProp Σ :=
     MonPred (λ V,
-      ⌜ Objective Φc ⌝ ∗
+      (* ⌜ Objective Φc ⌝ ∗ *)
       ∀ TV,
         ⌜V ⊑ TV⌝ -∗
         validV (store_view TV) -∗
@@ -16,7 +18,7 @@ Section wpc.
         WPC (ThreadState e TV) @ s; k; E {{ λ res,
           let '(ThreadVal v TV') := res return _ in
             validV (store_view TV') ∗ (Φ v TV') ∗ interp
-          }}{{ Φc TV }}
+          }}{{ Φc (∅, ∅, ∅) }}
     )%I _.
   Next Obligation. solve_proper. Qed.
 
@@ -28,14 +30,19 @@ Section wpc.
   Lemma wpc_eq : wpc = wpc_def.
   Proof. rewrite -wpc_aux.(seal_eq). done. Qed.
 
+  Global Instance wpc_ne s k E1 e n :
+    Proper (pointwise_relation _ (dist n) ==> dist n ==> dist n) (wpc s k E1 e).
+  Proof.
+    rewrite wpc_eq. constructor => V. solve_proper.
+  Qed.
+
   Lemma wpc_bind K s k E1 (e : expr) Φ Φc :
     WPC e @ s; k; E1 {{ v, WPC fill K (of_val v) @ s; k; E1 {{ Φ }} {{ Φc }} }} {{ Φc }}
                       ⊢ WPC fill K e @ s; k; E1 {{ Φ }} {{ Φc }}.
   Proof.
     rewrite wpc_eq.
     iStartProof (iProp _). iIntros (V).
-    iIntros "[#obj WP]".
-    iFrame "obj".
+    iIntros "WP".
     iIntros (TV) "incl val interp".
     iDestruct ("WP" with "incl val interp") as "HI".
     rewrite nvm_fill_fill.
@@ -43,14 +50,13 @@ Section wpc.
     { apply: ectx_lang_ctx. }
     iApply (wpc_mono with "HI").
     2: { done. }
-    iIntros ([v TV']) "(val & [obj wpc] & interp)".
+    iIntros ([v TV']) "(val & wpc & interp)".
     iDestruct ("wpc" $! TV' with "[//] val interp") as "HI".
     rewrite nvm_fill_fill.
     simpl. rewrite /thread_of_val. simpl.
-    iDestruct "obj" as %obj.
     iApply (wpc_crash_mono with "[] HI").
     iModIntro.
-    iApply objective_at.
+    iIntros "$".
   Qed.
 
 End wpc.
